Proofs/Experiments/AddLoop.lean
@@ -1,0 +1,655 @@
+/-
+Copyright (c) 2024 Amazon.com, Inc. or its affiliates. All Rights Reserved.
+Released under Apache 2.0 license as described in the file LICENSE.
+Author(s): Shilpi Goel
+
+Experimental: Use the Correctness module to prove that this program computes the
+following via a naive loop that iterates over `x0`:
+`x0 := x0 + x1`
+-/
+import Arm
+import Tactics.StepThms
+import Tactics.Sym
+import Correctness.ArmSpec
+
+namespace AddLoop
+
+/-
+Here is a C snippet that describes this program's behavior.
+
+while (x0 != 0) {
+  x1 := x1 + 1
+  x0 := x0 - 1
+}
+x0 := x1
+-/
+def program : Program :=
+    def_program
+    [
+      /- 00000000004005a4 <incr_test>:                             -/
+      (0x4005a4#64, 0x14000003#32), /- b        4005b0 <loop_test> -/
+
+      /- 00000000004005a8 <loop>:                                  -/
+      (0x4005a8#64, 0x91000421#32), /- add      x1, x1, #0x1       -/
+      (0x4005ac#64, 0xd1000400#32), /- sub      x0, x0, #0x1       -/
+
+      /- 00000000004005b0 <loop_test>:                              -/
+      (0x4005b0#64, 0xf100001f#32), /- cmp      x0, #0x0            -/
+      (0x4005b4#64, 0x54ffffa1#32), /- b.ne     4005a8 <loop>       -/
+      (0x4005b8#64, 0xaa0103e0#32), /- mov      x0, x1              -/
+      (0x4005bc#64, 0xd65f03c0#32)  /- ret                          -/
+      ]
+
+/-- Precondition for the correctness of the Add program. -/
+def pre (s : ArmState) : Prop :=
+  read_pc s = 0x4005a4#64 ∧
+  s.program = program ∧
+  read_err s = StateError.None ∧
+  -- (FIXME) We don't really need the stack pointer to be aligned, but the
+  -- `sym1_n` tactic expects this. Can we make this optional?
+  CheckSPAlignment s
+
+/-- Specification function. -/
+def spec (x0 x1 : BitVec 64) : BitVec 64 :=
+  x0 + x1
+
+def post (s0 sf : ArmState) : Prop :=
+  read_gpr 64 0#5 sf = spec (read_gpr 64 0#5 s0) (read_gpr 64 1#5 s0) ∧
+  read_pc sf = 0x4005bc#64 ∧
+  read_err sf = StateError.None ∧
+  sf.program = program ∧
+  -- (FIXME) We don't really need the stack pointer to be aligned, but the
+  -- `sym1_n` tactic expects this. Can we make this optional?
+  CheckSPAlignment sf
+
+def exit (s : ArmState) : Prop :=
+  -- (FIXME) Let's consider the state where we are poised to execute `ret` as an
+  -- exit state for now.
+  read_pc s = 0x4005bc#64
+
+def cut (s : ArmState) : Bool :=
+  -- First instruction
+  read_pc s = 0x4005a4#64 ||
+  -- Loop guard (branch instruction)
+  read_pc s = 0x4005b4#64 ||
+  -- First instruction following the loop
+  read_pc s = 0x4005b8#64 ||
+  -- Last instruction
+  read_pc s = 0x4005bc#64
+
+def loop_inv (s0 si : ArmState) : Prop :=
+  let x0 := read_gpr 64 0#5 s0
+  let x1 := read_gpr 64 1#5 s0
+  let curr_x0 := read_gpr 64 0#5 si
+  let curr_x1 := read_gpr 64 1#5 si
+  let curr_zf := r (StateField.FLAG PFlag.Z) si
+  (curr_x0 <= x0) ∧
+  ((curr_zf = 1#1) ↔ (curr_x0 = 0#64)) ∧
+  (curr_x1 = x1 + (x0 - curr_x0)) ∧
+  read_err si = .None ∧
+  si.program = program ∧
+  -- (FIXME) We don't really need the stack pointer to be aligned, but the
+  -- `sym1_n` tactic expects this. Can we make this optional?
+  CheckSPAlignment si
+
+def loop_post (s0 si : ArmState) : Prop :=
+  read_gpr 64 1#5 si = spec (read_gpr 64 0#5 s0) (read_gpr 64 1#5 s0) ∧
+  read_err si = .None ∧
+  si.program = program ∧
+  -- (FIXME) We don't really need the stack pointer to be aligned, but the
+  -- `sym1_n` tactic expects this. Can we make this optional?
+  CheckSPAlignment si
+
+def assert (s0 si : ArmState) : Prop :=
+  pre s0 ∧
+  -- Using `match` is preferable to `if` for the `split` tactic (and for
+  -- readability).
+  match (read_pc si) with
+  | 0x4005a4#64 =>
+    -- First instruction
+    si = s0
+  | 0x4005b4#64 =>
+    -- Loop guard
+    loop_inv s0 si
+  | 0x4005b8#64 =>
+    -- First instruction following the loop
+    loop_post s0 si
+  | 0x4005bc#64 =>
+    -- Last instruction
+    post s0 si
+  | _ => False
+
+instance : Spec' ArmState where
+  pre    := pre
+  post   := post
+  exit   := exit
+  cut    := cut
+  assert := assert
+
+theorem AddLoop.csteps_eq (s : ArmState) (i : Nat) :
+  Correctness.csteps s i = if cut s then i
+                           else Correctness.csteps (run 1 s) (i + 1) := by
+  rw [Correctness.csteps_eq]
+  simp only [Sys.next, Spec'.cut, run]
+  done
+
+-------------------------------------------------------------------------------
+-- Generating the program effects and non-effects
+
+-- set_option trace.gen_step.print_names true in
+#genStepTheorems program thmType:="fetch"
+-- set_option trace.gen_step.print_names true in
+#genStepTheorems program thmType:="decodeExec"
+-- set_option trace.gen_step.print_names true in
+#genStepTheorems program thmType:="step" `state_simp_rules
+
+-- (FIXME) Obtain *_cut theorems for each instruction automatically.
+
+theorem program.stepi_0x4005a4_cut (s sn : ArmState)
+  (h_program : s.program = program)
+  (h_pc : r StateField.PC s = 0x4005a4#64)
+  (h_err : r StateField.ERR s = StateError.None)
+  (h_sp_aligned : CheckSPAlignment s)
+  (h_step : sn = run 1 s) :
+  cut sn = false ∧
+  r StateField.PC sn = 0x4005b0#64 ∧
+  r StateField.ERR sn = .None ∧
+  sn.program = program ∧
+  CheckSPAlignment sn := by
+  have := program.stepi_0x4005a4 s (stepi s) h_program h_pc h_err
+  simp only [minimal_theory] at this
+  simp_all only [run, cut, this,
+                 state_simp_rules, bitvec_rules, minimal_theory]
+  done
+
+theorem program.stepi_0x4005a8_cut (s sn : ArmState)
+  (h_program : s.program = program)
+  (h_pc : r StateField.PC s = 0x4005a8#64)
+  (h_err : r StateField.ERR s = StateError.None)
+  (h_sp_aligned : CheckSPAlignment s)
+  (h_step : sn = run 1 s) :
+  cut sn = false ∧
+  r StateField.PC sn = 0x4005ac#64 ∧
+  r StateField.ERR sn = .None ∧
+  sn.program = program ∧
+  CheckSPAlignment sn := by
+  have := program.stepi_0x4005a8 s (stepi s) h_program h_pc h_err
+  simp only [minimal_theory, bitvec_rules] at this
+  simp_all only [run, cut, this, state_simp_rules, bitvec_rules, minimal_theory]
+  done
+
+theorem program.stepi_0x4005ac_cut (s sn : ArmState)
+  (h_program : s.program = program)
+  (h_pc : r StateField.PC s = 0x4005ac#64)
+  (h_err : r StateField.ERR s = StateError.None)
+  (h_sp_aligned : CheckSPAlignment s)
+  (h_step : sn = run 1 s) :
+  cut sn = false ∧
+  r StateField.PC sn = 0x4005b0#64 ∧
+  r StateField.ERR sn = .None ∧
+  sn.program = program ∧
+  CheckSPAlignment sn := by
+  have := program.stepi_0x4005ac s (run 1 s) h_program h_pc h_err
+  simp only [minimal_theory] at this
+  simp_all only [run, cut, this, state_simp_rules, bitvec_rules, minimal_theory]
+  done
+
+theorem program.stepi_0x4005b0_cut (s sn : ArmState)
+  (h_program : s.program = program)
+  (h_pc : r StateField.PC s = 0x4005b0#64)
+  (h_err : r StateField.ERR s = StateError.None)
+  (h_sp_aligned : CheckSPAlignment s)
+  (h_step : sn = run 1 s) :
+  cut sn = true ∧
+  r StateField.PC sn = 0x4005b4#64 ∧
+  r StateField.ERR sn = .None ∧
+  sn.program = program ∧
+  CheckSPAlignment sn := by
+  have := program.stepi_0x4005b0 s (run 1 s) h_program h_pc h_err
+  simp only [minimal_theory] at this
+  simp_all only [run, cut, this, state_simp_rules, bitvec_rules, minimal_theory]
+  done
+
+-- Branch instruction!
+theorem program.stepi_0x4005b4_cut (s sn : ArmState)
+  (h_program : s.program = program)
+  (h_pc : r StateField.PC s = 0x4005b4#64)
+  (h_err : r StateField.ERR s = StateError.None)
+  (h_sp_aligned : CheckSPAlignment s)
+  (h_step : sn = run 1 s) :
+  cut sn = (r (StateField.FLAG PFlag.Z) s = 1#1) ∧
+  r StateField.PC sn = (if (r (StateField.FLAG PFlag.Z) s = 1#1) then
+                                  0x4005b8#64
+                              else
+                                  0x4005a8#64) ∧
+  r StateField.ERR sn = .None ∧
+  sn.program = program ∧
+  CheckSPAlignment sn := by
+  have := program.stepi_0x4005b4 s (run 1 s) h_program h_pc h_err
+  simp only [minimal_theory] at this
+  simp_all only [run, cut, this, state_simp_rules, bitvec_rules, minimal_theory]
+  split
+  · rename_i h
+    simp_all only [state_simp_rules, bitvec_rules, minimal_theory]
+
+  · rename_i h; simp only [minimal_theory] at h
+    simp_all only [state_simp_rules, minimal_theory]
+    done
+
+theorem program.stepi_0x4005b8_cut (s sn : ArmState)
+  (h_program : s.program = program)
+  (h_pc : r StateField.PC s = 0x4005b8#64)
+  (h_err : r StateField.ERR s = StateError.None)
+  (h_sp_aligned : CheckSPAlignment s)
+  (h_step : sn = run 1 s) :
+  cut sn = true ∧
+  r StateField.PC sn = 0x4005bc#64 ∧
+  r StateField.ERR sn = .None ∧
+  sn.program = program ∧
+  CheckSPAlignment sn := by
+  have := program.stepi_0x4005b8 s (run 1 s) h_program h_pc h_err
+  simp only [minimal_theory] at this
+  simp_all only [run, cut, this, state_simp_rules, bitvec_rules, minimal_theory]
+  done
+
+-- (TODO) program.stepi_0x4005bc_cut elided.
+
+-------------------------------------------------------------------------------
+
+private theorem AddWithCarry.all_ones_identity_64 (x : BitVec 64) :
+  (AddWithCarry x 0xffffffffffffffff#64 0x1#1).fst = x := by
+  simp only [AddWithCarry]
+  bv_decide
+
+private theorem AddWithCarry.all_ones_zero_flag_64 (x : BitVec 64) :
+  ((AddWithCarry x 0xffffffffffffffff#64 0x1#1).snd.z = 1#1) ↔
+  (x = 0#64) := by
+  simp only [AddWithCarry, bitvec_rules, state_simp_rules]
+  repeat split
+  · bv_decide
+  · bv_decide
+  done
+
+theorem nextc_to_run_from_0x4005a4 (h : pre s0) :
+  (Correctness.nextc (Sys.run s0 1)) = run 2 s0 := by
+  simp only [pre, state_simp_rules] at h
+  obtain ⟨h_s0_pc, h_s0_program, h_s0_err⟩ := h
+  simp only
+    [Correctness.nextc, Correctness.arm_run,
+     Spec'.cut, minimal_theory]
+
+  rw [AddLoop.csteps_eq]
+  have h_step_1 := program.stepi_0x4005a4_cut s0 (run 1 s0)
+  simp_all only [minimal_theory, bitvec_rules]
+  generalize h_s1 : run 1 s0 = s1 at h_step_1
+
+  -- Stop when the *_cut theorem says (cut <state>) = true.
+  rw [AddLoop.csteps_eq]
+  have h_step_2 := program.stepi_0x4005b0_cut s1 (run 1 s1)
+  simp_all only [minimal_theory]
+  generalize h_s2 : run 1 s1 = s2 at h_step_2
+
+  simp only [←h_s2, ←h_s1, ←run_plus]
+  done
+
+theorem effects_of_nextc_from_0x4005a4
+  (h_pre : pre s0)
+  (_h_pc : r StateField.PC s0 = 0x4005a4#64)
+  (h_run : sf = (Correctness.nextc (Sys.run s0 1))) :
+  -- I've elided irrelevant effects and non-effects for now.
+  sf.program = program ∧
+  r StateField.PC sf = 0x4005b4#64 ∧
+  r StateField.ERR sf = .None ∧
+  ((r (StateField.FLAG PFlag.Z) sf = 1#1) ↔
+   (r (StateField.GPR 0x0#5) s0 = 0x0#64)) ∧
+  r (StateField.GPR 0#5) sf = r (StateField.GPR 0#5) s0 ∧
+  r (StateField.GPR 1#5) sf = r (StateField.GPR 1#5) s0 ∧
+  CheckSPAlignment sf := by
+  -- Prelude
+  rw [nextc_to_run_from_0x4005a4 h_pre] at h_run
+  -- TODO: Tactic to "explode" conjunctions?
+  obtain ⟨h_s0_pc, h_s0_program, h_s0_err, h_s0_sp_aligned⟩ := h_pre
+  -- Symbolic simulation
+  -- (FIXME) sym1_n doesn't play well with unconditional branches.
+  /-
+  application type mismatch
+  program.stepi_0x4005a8 s1 s2 h_s1_program h_s1_pc
+  argument
+  h_s1_pc
+  has type
+  r StateField.PC s1 = 0x4005b0#64 : Prop
+  but is expected to have type
+  r StateField.PC s1 = 0x4005a8#64 : Prop
+  -/
+  -- sym1_n 2
+  sym1_n 1 at s0
+  sym1_n 1 at s1
+  -- (FIXME) better stepi lemma generation
+  simp (config := {ground := true}) only at h_step_2
+  -- Aggregate block effects
+  -- explode_step h_step_1
+  -- explode_step h_step_2
+  simp only [run] at h_run
+  subst h_run
+  simp only [*, state_simp_rules, bitvec_rules, minimal_theory]
+  rw [AddWithCarry.all_ones_zero_flag_64]
+  done
+
+-------------------------------------------------------------------------------
+
+theorem nextc_to_run_from_0x4005b4_cond_holds_true (_h_pre : pre s0)
+  (h_pc : r StateField.PC si = 0x4005b4#64)
+  (h_cond_holds_true : r (StateField.FLAG PFlag.Z) si = 0#1)
+  (h_inv : loop_inv s0 si) :
+  (Correctness.nextc (Sys.run si 1)) = run 4 si := by
+  simp only [pre, loop_inv, state_simp_rules] at *
+  obtain ⟨_h_inv_x0_le, h_inv_z, h_inv_x1, h_inv_err,
+          h_inv_program, h_inv_sp_aligned⟩ := h_inv
+  simp only
+    [Correctness.nextc, Correctness.arm_run,
+     Spec'.cut, minimal_theory]
+
+  rw [AddLoop.csteps_eq]
+  have h_step_1 := program.stepi_0x4005b4_cut si (run 1 si)
+  simp_all only [minimal_theory, bitvec_rules]
+  -- (FIXME) Why do we need this decide?
+  simp (config := {decide := true}) only [*, minimal_theory] at h_inv_z
+  simp_all only [h_inv_z, minimal_theory]
+  --
+  generalize h_s1 : run 1 si = s1 at h_step_1
+
+  rw [AddLoop.csteps_eq]
+  have h_step_2 := program.stepi_0x4005a8_cut s1 (run 1 s1)
+  simp_all only [minimal_theory, bitvec_rules]
+  generalize h_s2 : run 1 s1 = s2 at h_step_2
+
+  rw [AddLoop.csteps_eq]
+  have h_step_3 := program.stepi_0x4005ac_cut s2 (run 1 s2)
+  simp_all only [minimal_theory, bitvec_rules]
+  generalize h_s3 : run 1 s2 = s3 at h_step_3
+
+  -- Stop when the *_cut theorem says (cut <state>) = true.
+  rw [AddLoop.csteps_eq]
+  have h_step_4 := program.stepi_0x4005b0_cut s3 (run 1 s3)
+  simp_all only [minimal_theory, bitvec_rules]
+  generalize h_s4 : run 1 s3 = s4 at h_step_4
+
+  -- (FIXME): Ugh, obtaining the intermediate states in terms of each other and
+  -- the initial states is such a pain!
+  have h_s4_s1 : s4 = run 3 s1 := by
+    simp only [←h_s4, ←h_s3, ←run_plus, ←h_s2,
+                minimal_theory, bitvec_rules]
+  simp only [←h_s4_s1, h_step_4,
+              bitvec_rules, minimal_theory]
+  simp only [h_s4_s1, ←h_s1, ←run_plus]
+  done
+
+private theorem non_zero_one_bit_is_one (x : BitVec 1)
+  (h : ¬ x = 0#1) :
+  x = 1#1 := by
+  bv_decide
+
+theorem nextc_to_run_from_0x4005b4_cond_holds_false (_h_pre : pre s0)
+  (h_pc : r StateField.PC si = 0x4005b4#64)
+  (h_cond_holds_false : ¬ (r (StateField.FLAG PFlag.Z) si = 0#1))
+  (h_inv : loop_inv s0 si) :
+  (Correctness.nextc (Sys.run si 1)) = run 1 si := by
+  simp only [pre, loop_inv, state_simp_rules] at *
+  obtain ⟨_h_inv_x0_le, h_inv_z, h_inv_x1, h_inv_err,
+          h_inv_program, h_inv_sp_aligned⟩ := h_inv
+  simp only
+    [Correctness.nextc, Correctness.arm_run,
+     Spec'.cut, minimal_theory]
+
+  -- Stop when the *_cut theorem says (cut <state>) = true.
+  rw [AddLoop.csteps_eq]
+  have h_step_1 := program.stepi_0x4005b4_cut si (run 1 si)
+  simp_all only [non_zero_one_bit_is_one, minimal_theory, bitvec_rules]
+  generalize _h_s1 : run 1 si = s1 at h_step_1
+
+  simp only [run, h_step_1, minimal_theory]
+  done
+
+private theorem AddWithCarry.sub_one_64 (x : BitVec 64) :
+  (AddWithCarry x 0xfffffffffffffffe#64 0x1#1).fst = x - 1#64 := by
+  simp only [AddWithCarry]
+  bv_decide
+
+theorem effects_of_nextc_from_0x4005b4_cond_holds_true
+  (h_pre : pre s0)
+  (h_pc : r StateField.PC si = 0x4005b4#64)
+  (h_cond_holds_true : r (StateField.FLAG PFlag.Z) si = 0#1)
+  (h_inv : loop_inv s0 si)
+  (h_run : sf = (Correctness.nextc (Sys.run si 1))) :
+  r (StateField.GPR 0#5) sf = r (StateField.GPR 0x0#5) si - 0x1#64 ∧
+  r (StateField.GPR 1#5) sf =
+      (AddWithCarry (r (StateField.GPR 0x1#5) s0 +
+                    (r (StateField.GPR 0x0#5) s0 -
+                    r (StateField.GPR 0x0#5) si))
+                    0x1#64
+                    0x0#1).fst ∧
+  r (StateField.FLAG PFlag.Z) sf =
+    (AddWithCarry (r (StateField.GPR 0x0#5) si - 0x1#64)
+                  0xffffffffffffffff#64 0x1#1).snd.z ∧
+  r StateField.PC sf = 0x4005b4#64 ∧
+  r StateField.ERR sf = .None ∧
+  sf.program = program ∧
+  CheckSPAlignment sf := by
+  -- Prelude
+  rw [nextc_to_run_from_0x4005b4_cond_holds_true
+       h_pre h_pc h_cond_holds_true h_inv] at h_run
+  simp only [state_simp_rules, loop_inv] at h_inv
+  obtain ⟨_h_inv_x0_le, h_inv_z, h_inv_x1, h_inv_err,
+          h_inv_program, h_inv_sp_aligned⟩ := h_inv
+  simp (config := {decide := true}) only
+    [h_cond_holds_true, minimal_theory] at h_inv_z
+  -- Symbolic simulation
+  -- (TODO) Better handling for branch instructions.
+  init_next_step h_run h_step_1 s1
+  rw [program.stepi_0x4005b4] at h_step_1
+  simp only [*, bitvec_rules, minimal_theory] at h_step_1
+  (intro_fetch_decode_lemmas h_step_1 h_inv_program "h_inv";
+   all_goals (try assumption))
+  --
+  sym1_n 3 at s1
+  -- Aggregating the effects
+  simp (config := {ground := true}) only
+    at h_step_2 h_step_3 h_step_4
+  simp only [run] at h_run
+  simp only [*, AddWithCarry.sub_one_64,
+    state_simp_rules, bitvec_rules, minimal_theory]
+  done
+
+theorem effects_of_nextc_from_0x4005b4_cond_holds_false
+  (h_pre : pre s0)
+  (h_pc : r StateField.PC si = 0x4005b4#64)
+  (h_cond_holds_false : ¬ (r (StateField.FLAG PFlag.Z) si = 0#1))
+  (h_inv : loop_inv s0 si)
+  (h_run : sf = (Correctness.nextc (Sys.run si 1))) :
+  r (StateField.GPR 0#5) sf = 0#64 ∧
+  r (StateField.GPR 1#5) sf =
+      r (StateField.GPR 0x1#5) s0 + r (StateField.GPR 0x0#5) s0 ∧
+  r (StateField.FLAG PFlag.Z) sf = 1#1 ∧
+  r StateField.PC sf = 0x4005b8#64 ∧
+  r StateField.ERR sf = .None ∧
+  sf.program = program ∧
+  CheckSPAlignment sf := by
+  -- Prelude
+  rw [nextc_to_run_from_0x4005b4_cond_holds_false
+       h_pre h_pc h_cond_holds_false h_inv] at h_run
+  simp only [state_simp_rules, loop_inv] at h_inv
+  obtain ⟨_h_inv_x0_le, h_inv_z, h_inv_x1, h_inv_err,
+          h_inv_program, h_inv_sp_aligned⟩ := h_inv
+  simp (config := {decide := true}) only
+    [non_zero_one_bit_is_one, h_cond_holds_false, minimal_theory] at h_inv_z
+  -- Symbolic simulation
+  -- sym1_n 1 at si
+  -- (TODO) Better handling for branch instructions.
+  init_next_step h_run h_step_1 s1
+  rw [program.stepi_0x4005b4] at h_step_1
+  simp only [*, non_zero_one_bit_is_one, bitvec_rules, minimal_theory]
+    at h_step_1
+  (intro_fetch_decode_lemmas h_step_1 h_inv_program "h_inv";
+   all_goals (try assumption))
+  -- Aggregating the effects
+  simp only [run] at h_run
+  simp only [*, non_zero_one_bit_is_one,
+              state_simp_rules, bitvec_rules, minimal_theory]
+  done
+
+-------------------------------------------------------------------------------
+
+theorem nextc_to_run_from_0x4005b8 (_h_pre : pre s0)
+  (h_pc : r StateField.PC si = 0x4005b8#64)
+  (h_assert : loop_post s0 si) :
+  Correctness.nextc (Sys.run si 1) = run 1 si := by
+  simp only [pre, loop_post, state_simp_rules] at *
+  obtain ⟨_h_inv_x0, h_inv_err, h_inv_program, h_inv_sp_aligned⟩ := h_assert
+
+  simp only
+    [Correctness.nextc, Correctness.arm_run,
+     Spec'.cut, minimal_theory]
+
+  -- Stop when the *_cut theorem says (cut <state>) = true.
+  rw [AddLoop.csteps_eq]
+  have h_step_1 := program.stepi_0x4005b8_cut si (run 1 si)
+  simp_all only [minimal_theory, bitvec_rules]
+  generalize _h_s1 : run 1 si = s1 at h_step_1
+
+  simp only [run_opener_zero, h_step_1, minimal_theory]
+  done
+
+theorem effects_of_nextc_from_0x4005b8 (_h_pre : pre s0)
+  (h_pc : r StateField.PC si = 0x4005b8#64)
+  (h_assert : loop_post s0 si)
+  (h_run : sf = Correctness.nextc (Sys.run si 1)) :
+  r (StateField.GPR 0#5) sf = r (StateField.GPR 1#5) si ∧
+  r StateField.PC sf = 0x4005bc#64 ∧
+  r StateField.ERR sf = .None ∧
+  sf.program = program ∧
+  CheckSPAlignment sf := by
+  -- Prelude
+  rw [nextc_to_run_from_0x4005b8 _h_pre h_pc h_assert] at h_run
+  -- TODO: Tactic to "explode" conjunctions?
+  obtain ⟨_h_inv_x0, h_inv_err, h_inv_program, h_inv_sp_aligned⟩ := h_assert
+  -- Symbolic simulation
+  -- TODO: Why do we need `try assumption` here?
+  sym1_n 1 at si <;> try assumption
+  -- Aggregate effects.
+  simp only [run] at h_run
+  subst h_run
+  simp only [*, state_simp_rules, bitvec_rules, minimal_theory]
+  done
+
+-------------------------------------------------------------------------------
+
+-- TODO: Upstream?
+@[bitvec_rules]
+theorem BitVec.le_refl (x : BitVec n) :
+  x <= x := by
+  exact BitVec.le_of_eq x x rfl
+
+private theorem loop_inv_x0_le (x y : BitVec 64)
+  (h_assert_x0 : x ≤ y)
+  (h_assert_x0_nz : ¬x = 0x0#64) :
+  x - 0x1#64 ≤ y := by
+  bv_omega
+
+private theorem AddWithCarry.add_one_64 (x : BitVec 64) :
+  (AddWithCarry x 0x1#64 0x0#1).fst = x + 0x1#64 := by
+  simp only [AddWithCarry, bitvec_rules]
+  bv_omega
+
+private theorem crock_lemma (x y z : BitVec 64) :
+  x + (y - z) + 1#64 = x + (y - (z - 1#64)) := by
+  -- (FIXME) Without this apply below, bv_omega crashes my editor.
+  apply BitVec.eq_sub_iff_add_eq.mp
+  bv_omega
+
+theorem partial_correctness :
+  PartialCorrectness ArmState := by
+  apply Correctness.partial_correctness_from_verification_conditions
+  case v1 =>
+    intro s0 h_pre
+    simp_all only [Spec.pre, pre, Spec'.assert, assert,
+                    minimal_theory]
+  case v2 =>
+    intro sf h_exit
+    simp_all only [Spec.exit, exit, Spec'.cut, cut,
+                    state_simp_rules, minimal_theory]
+  case v3 =>
+    intro s0 sf h_assert h_exit
+    -- (FIXME) Remove Spec.post to replicate bug where simp_all somehow
+    -- aggressively makes the goal unprovable.
+    simp_all only [Spec'.assert, Spec.exit, assert, exit, Spec.post]
+  case v4 =>
+    intro s0 si h_assert h_exit
+    simp_all only [Spec'.assert, Spec.exit, assert, exit,
+                   minimal_theory, state_simp_rules]
+    obtain ⟨h_pre, h_assert⟩ := h_assert
+    split at h_assert
+    · -- Next cutpoint from 0x4005a4#64 (first instruction)
+      generalize h_sn : (Correctness.nextc (Sys.run si 1)) = sn
+      subst h_assert
+      simp_all only [bitvec_rules, minimal_theory]
+      have h_effects := @effects_of_nextc_from_0x4005a4 si sn
+      simp only [*, minimal_theory] at h_effects
+      simp only [h_effects, loop_inv,
+                 state_simp_rules, bitvec_rules, minimal_theory]
+      done
+    · -- Next cutpoint from 0x4005b4#64 (loop guard)
+      generalize h_sn : (Correctness.nextc (Sys.run si 1)) = sn
+      by_cases h_cond_holds : r (StateField.FLAG PFlag.Z) si = 0x0#1
+      case pos =>
+        have h_effects :=
+          @effects_of_nextc_from_0x4005b4_cond_holds_true s0 si sn
+        simp only [*, minimal_theory] at h_effects
+        simp only [*, loop_inv,
+                   state_simp_rules, bitvec_rules, minimal_theory]
+        simp (config := {decide := true}) only
+                  [loop_inv, h_cond_holds, non_zero_one_bit_is_one,
+                   state_simp_rules, bitvec_rules, minimal_theory]
+          at h_assert
+        obtain ⟨h_assert_x0, h_assert_x0_nz, _h_assert_x1, _, _, _⟩ := h_assert
+        apply And.intro
+        · apply loop_inv_x0_le
+                (r (StateField.GPR 0x0#5) si) (r (StateField.GPR 0x0#5) s0)
+                h_assert_x0 h_assert_x0_nz
+        · apply And.intro
+          · apply AddWithCarry.all_ones_zero_flag_64
+          · simp only [AddWithCarry.add_one_64]
+            rw [crock_lemma]
+      case neg =>
+        have h_effects :=
+          @effects_of_nextc_from_0x4005b4_cond_holds_false s0 si sn
+        simp only [*, minimal_theory] at h_effects
+        simp only [*, loop_post, spec,
+                   minimal_theory, bitvec_rules, state_simp_rules]
+        ac_rfl
+        done
+    · -- Next cutpoint from 0x4005b8#64 (first instruction after loop)
+      generalize h_sn : (Correctness.nextc (Sys.run si 1)) = sn
+      have h_effects := @effects_of_nextc_from_0x4005b8 s0 si sn
+      simp only [*, minimal_theory] at h_effects
+      simp only [h_effects, post,
+                 state_simp_rules, bitvec_rules, minimal_theory]
+      simp only [loop_post,
+                  state_simp_rules, bitvec_rules, minimal_theory]
+        at h_assert
+      simp_all only
+      done
+    · -- Next cutpoint from 0x4005bc#64 (last instruction)
+      -- No such cutpoint exists:
+      contradiction
+    · -- No further cutpoints exist.
+      simp_all only
+  done
+
+theorem termination :
+  Termination ArmState := by
+  simp [Termination, Spec.pre, Spec.exit, exit,
+        state_simp_rules, bitvec_rules, minimal_theory]
+  intro s h_pre
+  sorry
+
+end AddLoop
